DLM sa -> ip

aneris/examples/reliable_communication/lib/dlm/dlm_spec.v
@@ -6,8 +6,8 @@ From aneris.examples.reliable_communication.spec Require Import resources.
 From aneris.examples.reliable_communication.lib.dlm Require Import dlm_code dlm_prelude.
 
 Class DL_resources `{!anerisG Mdl Σ} := {
-    DLockCanAcquire : socket_address → val → iProp Σ → iProp Σ;
-    DLockCanRelease : socket_address → val → iProp Σ → iProp Σ;
+    DLockCanAcquire : ip_address → val → iProp Σ → iProp Σ;
+    DLockCanRelease : ip_address → val → iProp Σ → iProp Σ;
     dl_service_init : iProp Σ;
     dl_service_init_exclusive : dl_service_init -∗ dl_service_init -∗ False;
     dl_service_init_timeless :> Timeless (dl_service_init);
@@ -31,15 +31,15 @@ Section DL_spec.
       dlock_start_service #srv_sa @[srv_ip]
     {{{ RET #(); True }}}.
 
-  Definition dl_acquire_spec (sa : socket_address) (dl : val) : iProp Σ :=
-    {{{ DLockCanAcquire sa dl R  }}}
-       dlock_acquire dl @[ip_of_address sa]
-     {{{ RET #(); DLockCanRelease sa dl R ∗ R }}}.
+  Definition dl_acquire_spec (ip : ip_address) (dl : val) : iProp Σ :=
+    {{{ DLockCanAcquire ip dl R  }}}
+       dlock_acquire dl @[ip]
+     {{{ RET #(); DLockCanRelease ip dl R ∗ R }}}.
 
-  Definition dl_release_spec (sa : socket_address) (dl : val) : iProp Σ :=
-    {{{ DLockCanRelease sa dl R ∗ R }}}
-       dlock_release dl @[ip_of_address sa]
-    {{{ RET #(); DLockCanAcquire sa dl R }}}.
+  Definition dl_release_spec (ip : ip_address) (dl : val) : iProp Σ :=
+    {{{ DLockCanRelease ip dl R ∗ R }}}
+       dlock_release dl @[ip]
+    {{{ RET #(); DLockCanAcquire ip dl R }}}.
 
   Definition dl_subscribe_client_spec : iProp Σ :=
     ∀ (sa : socket_address) A,
@@ -47,8 +47,9 @@ Section DL_spec.
         free_ports (ip_of_address sa) {[port_of_address sa]} ∗ sa ⤳ (∅, ∅) ∗
          DL_server_addr ⤇ dl_reserved_server_socket_interp }}}
       dlock_subscribe_client #sa #srv_sa @[ip_of_address sa]
-      {{{ dl, RET dl; DLockCanAcquire sa dl R ∗
-                      dl_acquire_spec sa dl ∗ dl_release_spec sa dl }}}.
+      {{{ dl, RET dl; DLockCanAcquire (ip_of_address sa) dl R ∗
+                      dl_acquire_spec (ip_of_address sa) dl ∗
+                      dl_release_spec (ip_of_address sa) dl }}}.
 
 End DL_spec.
 
